src/mqtt-packet-parser/src/debug_ffi.c
@@ -4,3 +4,14 @@
 void print_hex(uint8_t i) {
   printf("%02x", i);
 }
+
+void print_buffer(uint8_t *buffer, uint32_t buffer_size) {
+  printf("[");
+  for (int i = 0; i < buffer_size; i++)
+  {
+    printf("%02x", buffer[i]);
+    if (i != buffer_size - 1)
+      printf(", ");
+  }
+  puts("]");
+}
