src/mqtt-packet-parser/src/const.fst
@@ -262,6 +262,7 @@ type struct_variable_header_publish = {
   topic_name: type_topic_name_restrict;
   property_length: type_property_length;
   payload: type_payload_restrict;
+  payload_length: U32.t;
   property_id: U8.t;
 }
 
@@ -612,6 +613,7 @@ type struct_publish_parts = {
   publish_topic_length: type_topic_length_restrict;
   publish_property_length: type_property_length;
   publish_payload: type_payload_restrict;
+  publish_payload_length: U32.t;
   publish_property_id: U8.t;
 }
 
@@ -657,6 +659,7 @@ type struct_publish_packet_seed = {
   publish_seed_is_searching_property_length: bool;
   publish_seed_property_length: type_property_length;
   publish_seed_payload: type_payload_restrict;
+  publish_seed_payload_length: U32.t;
   publish_seed_payload_error_status: U8.t;
   publish_seed_property_id: U8.t;
 }
@@ -689,4 +692,5 @@ type struct_property = {
 type struct_payload = {
   is_valid_payload: bool;
   payload: B.buffer U8.t;
+  payload_length: U32.t;
 }
