src/mqtt-packet-parser/src/debug_ffi.fst
@@ -1,9 +1,17 @@
 module Debug_FFI
 
 module U8 = FStar.UInt8
+module U32 = FStar.UInt32
+module B = LowStar.Buffer
 
 open FStar.HyperStack.ST
 
 assume val print_hex (i:U8.t): Stack unit
+  (requires (fun h -> true))
+  (ensures (fun h0 ret h1 -> true))
+
+assume val print_buffer: (buffer: B.buffer U8.t)
+-> buffer_size: U32.t
+-> Stack unit
   (requires (fun h -> true))
   (ensures (fun h0 ret h1 -> true))
